2、因式分解
$x^{15}+x^{14}+x^{13}+x^{12}+x^{11}+x^{10}+x^9+x^8+x^7+x^6+x^5+x^4+x^3+x^2+x+1$
解:原式   $ =\left(x^{15}+x^{14} \right)+\left(x^{13}+x^{12} \right)\cdots\left(x+1 \right)$
                $ =x^{14}\left(x+1 \right)+x^{12}\left(x+1 \right)\cdots\left(x+1 \right)$
                $ = \left(x+1 \right)\left(x^{14}+x^{12}+x^{10}+x^8+x^6+x^4+x^2+1 \right)$
                $ = \left(x+1 \right)\left(x^2+1 \right)\left(x^{12}+x^8+x^4+1 \right)$
                $ = \left(x+1 \right)\left(x^2+1 \right)\left(x^4+1 \right)\left(x^8+1 \right)$



 已知$ x^2-5x=14 $，求$\left(x-1 \right)\left(2x-1 \right)-{\left(x+1 \right)}^2+1$的值



